replace old TaggedComp with TaggedComp2

src/TaggedComp.v
@@ -52,6 +52,7 @@ Definition compile (e : L.expr) : option T.expr :=
         | L.Close f free => T.Close f <$> go_list free
         end in go e.
 
+(* Nested fixpoint alias for `compile`, but also used as a top-level function *)
 Definition compile_list :=
     let fix go_list (es : list L.expr) : option (list T.expr) :=
         match es with
@@ -65,1636 +66,94 @@ Definition compile_program (lp : L.expr * list L.expr) : option (T.expr * list T
 End compile.
 
 
+(* spec *)
 
-(* Test compiler *)
-
-Eval compute in compile_program L.add_prog.
-
-Definition add_comp :=
-    let x := compile L.add_reflect in
-    match x as x_ return x = x_ -> _ with
-    | Some x => fun _ => x
-    | None => fun H => ltac:(discriminate)
-    end eq_refl.
-Definition add_env_comp :=
-    let x := compile_list L.add_env in
-    match x as x_ return x = x_ -> _ with
-    | Some x => fun _ => x
-    | None => fun H => ltac:(discriminate)
-    end eq_refl.
-
-Theorem add_1_2 :
-    { x | T.star add_env_comp
-        (T.Call (T.Call add_comp (T.nat_reflect 1)) (T.nat_reflect 2)) x }.
-eexists.
-
-unfold add_comp. simpl.
-eright. eapply T.CallL, T.MakeCall; try solve [repeat econstructor].
-eright. eapply T.MakeCall; try solve [repeat econstructor].
-eright. eapply T.CallL, T.Eliminate; try solve [repeat econstructor].
-eright. eapply T.CallL, T.CallL, T.MakeCall; try solve [repeat econstructor].
-eright. eapply T.CallL, T.CallR, T.Eliminate; try solve [repeat econstructor].
-eright. eapply T.CallL, T.MakeCall; try solve [repeat econstructor].
-eright. eapply T.MakeCall; try solve [repeat econstructor].
-eright. eapply T.MakeCall; try solve [repeat econstructor].
-eleft.
-Defined.
-Eval compute in proj1_sig add_1_2.
-
-(* end of test *)
-
-
-
-
-Inductive expr_ok : L.expr -> Prop :=
-| VArg : expr_ok L.Arg
-| VUpVar : forall n, expr_ok (L.UpVar n)
-| VCall : forall f a, expr_ok f -> expr_ok a -> expr_ok (L.Call f a)
-| VConstr : forall c args,
-        Utopia.constructor_arg_n c = length args ->
-        Forall expr_ok args ->
-        expr_ok (L.Constr c args)
-| VElim : forall ty cases target,
-        (forall i, i < length cases -> Utopia.type_constr ty i <> None) ->
-        Forall expr_ok cases ->
-        expr_ok target ->
-        expr_ok (L.Elim ty cases target)
-| VClose : forall f free,
-        Forall expr_ok free ->
-        expr_ok (L.Close f free)
-.
-
-Ltac generalize_all :=
-    repeat match goal with
-    | [ y : _ |- _ ] => generalize y; clear y
-    end.
-
-(* Change the current goal to an equivalent one in which argument "x" is the
- * first one. *)
-Tactic Notation "make_first" ident(x) :=
-    try intros until x;
-    move x at top;
-    generalize_all.
-
-(* Move "x" to the front of the goal, then perform induction. *)
-Ltac first_induction x := make_first x; induction x.
-
-Tactic Notation "intros0" ne_ident_list(xs) :=
-    intros until 0; intros xs.
-
-Notation "**" := (ltac:(eassumption)) (only parsing).
-Notation "??" := (ltac:(shelve)) (only parsing).
-
-Lemma cases_len_mk_tagged_cases' : forall ty idx cases len,
-    (forall i, i < len -> Utopia.type_constr ty i <> None) ->
-    idx + length cases = len ->
-    mk_tagged_cases' ty idx cases <> None.
-first_induction cases; intros0 Hok Hlen; simpl.
-{ discriminate. }
-compute [seq fmap bind_option]. simpl in Hlen.
-assert (idx < len) by omega.
-pose proof Hok. specialize (Hok _ **). break_match; try congruence.
-specialize (IHcases _ (S idx) _ ** ltac:(omega)). break_match; congruence.
-Qed.
-
-Lemma cases_len_mk_tagged_cases : forall ty cases,
-    (forall i, i < length cases -> Utopia.type_constr ty i <> None) ->
-    mk_tagged_cases ty cases <> None.
-intros. unfold mk_tagged_cases. eapply cases_len_mk_tagged_cases'; eauto.
-Qed.
-
-Lemma compile_list_len : forall es es',
-    compile_list es = Some es' ->
-    length es = length es'.
-induction es; intros0 Hcomp; simpl in *.
-- injection Hcomp. intro HH. rewrite <- HH. reflexivity.
-- compute [seq fmap bind_option] in Hcomp.
-  break_match; try discriminate.
-  break_match; try discriminate.
-  break_match; try discriminate.
-  invc Heqo. invc Hcomp. erewrite IHes; eauto. reflexivity.
-Qed.
-
-Theorem expr_ok_compile : forall e, expr_ok e -> compile e <> None.
-induction e using L.expr_rect_mut
-    with (Pl := fun es => Forall expr_ok es -> compile_list es <> None);
-    intros0 Hok; simpl.
-
-- discriminate.
-
-- discriminate.
-
-- compute [seq fmap bind_option].
-  invc Hok. specialize (IHe1 **). specialize (IHe2 **).
-  destruct (compile e1); try congruence.
-  destruct (compile e2); try congruence.
-
-- fold compile_list. compute [seq fmap bind_option].
-  invc Hok. specialize (IHe **).
-  break_match; congruence.
-
-- fold compile_list. compute [seq fmap bind_option].
-  invc Hok. specialize (IHe **). specialize (IHe0 **).
-  break_match; try congruence.
-  break_match; cycle 1.
-    { break_match; try discriminate.
-      contradict Heqo1. eapply cases_len_mk_tagged_cases.
-      intro. erewrite <- compile_list_len; eauto. }
-  break_match; try congruence.
-
-- fold compile_list. compute [seq fmap bind_option].
-  invc Hok. specialize (IHe **).
-  break_match; congruence.
-
-- discriminate.
-
-- compute [seq fmap bind_option].
-  invc Hok. specialize (IHe **). specialize (IHe0 **).
-  destruct (compile _); try congruence.
-  destruct (compile_list _); try congruence.
-
-Qed.
-
-
-
-
-Inductive match_states (LE : L.env) (TE : T.env) : L.expr -> T.expr -> Prop :=
-| MsArg :
-        match_states LE TE L.Arg T.Arg
-| MsUpVar : forall n,
-        match_states LE TE (L.UpVar n) (T.UpVar n)
-| MsCall : forall lf la tf ta,
-        match_states LE TE lf tf ->
-        match_states LE TE la ta ->
-        match_states LE TE (L.Call lf la) (T.Call tf ta)
-| MsConstr : forall c largs tag targs,
-        Utopia.constructor_index c = tag ->
-        Forall2 (match_states LE TE) largs targs ->
-        match_states LE TE (L.Constr c largs) (T.Constr tag targs)
-| MsElim : forall ty lcases ltarget tcases0 tcases ttarget,
-        Forall2 (match_states LE TE) lcases tcases0 ->
-        mk_tagged_cases ty tcases0 = Some tcases ->
-        match_states LE TE ltarget ttarget ->
-        match_states LE TE (L.Elim ty lcases ltarget) (T.Elim tcases ttarget)
-| MsClose : forall fn largs targs,
-        Forall2 (match_states LE TE) largs targs ->
-        match_states LE TE (L.Close fn largs) (T.Close fn targs)
-.
-
-
-
-
-
-
-
-Lemma match_value : forall LE TE le te,
-    match_states LE TE le te ->
-    L.value le ->
-    T.value te.
-induction le using L.expr_ind'; intros0 Hmatch Lval; invc Lval; invc Hmatch.
-
-- constructor.
-
-  assert (HH :
-  forall i,
-      forall arg, nth_error args i = Some arg ->
-      forall targ, nth_error targs i = Some targ ->
-      (forall te, match_states LE TE arg te -> L.value arg -> T.value te) ->
-      L.value arg ->
-      match_states LE TE arg targ ->
-      T.value targ
-  ) by (clear; intros; eauto).
-
-  list_magic **.
-
-- constructor.
-
-  assert (HH :
-  forall i,
-      forall arg, nth_error free i = Some arg ->
-      forall targ, nth_error targs i = Some targ ->
-      (forall te, match_states LE TE arg te -> L.value arg -> T.value te) ->
-      L.value arg ->
-      match_states LE TE arg targ ->
-      T.value targ
-  ) by (clear; intros; eauto).
-
-  list_magic **.
-Qed.
-
-Theorem match_step : forall LE TE le le' te,
-    Forall2 (match_states LE TE) LE TE ->
-    match_states LE TE le te ->
-    L.step LE le le' ->
-    exists te', T.step TE te te' /\ match_states LE TE le' te'.
-intros. move le at top. generalize_all.
-induction le using L.expr_ind'; intros0 Henv Hmatch Lstep; try solve [invc Lstep].
-
-- (* Call *)
-  invc Lstep.
-
-  + (* MakeCall *)
-    invc Hmatch. invc H4.
-
-    eexists. split.
-    -- fwd eapply Forall2_nth_error_Some with (xs := LE) (ys := TE); eauto.  break_exists.
-       eapply T.MakeCall; eauto using match_value.
-
-       ++ assert (forall i,
-            forall lv, nth_error free i = Some lv ->
-            forall tv, nth_error targs i = Some tv ->
-            match_states LE TE lv tv ->
-            L.value lv ->
-            T.value tv) by (eauto using match_value).
-          list_magic **.
-
-       ++ admit. (* T.subst succeeds because L.subst succeeds *)
-
-    -- admit. (* (1) needs subst/match lemma; (2) need to know how te' was made *)
-
-  + (* CallL *)
-    invc Hmatch.
-    fwd eapply IHle1; eauto. 
-    break_exists. break_and.
-    eexists. split; econstructor; eauto.
-
-  + (* CallR *)
-    invc Hmatch.
-    fwd eapply IHle2; eauto.
-    break_exists. break_and.
-    eexists. split; econstructor; solve [eauto using match_value].
-
-- (* Constr *)
-  invc Lstep. invc Hmatch.
-  admit.
-
-- admit.
-- admit.
-Admitted.
-
-Theorem match_star : forall LE TE le le',
-    Forall2 (match_states LE TE) LE TE ->
-    L.star LE le le' ->
-    forall te, match_states LE TE le te ->
-    exists te', T.star TE te te' /\ match_states LE TE le' te'.
-induction 2; intros.
-- exists te. split; [constructor | assumption].
-- fwd eapply match_step; eauto. break_exists. break_and.
-  fwd eapply IHstar; eauto. break_exists. break_and.
-  eexists. split; [ | eassumption ]. econstructor; eassumption.
-Qed.
-
-Theorem match_star_value : forall LE TE le le' te te',
-    Forall2 (match_states LE TE) LE TE ->
-    L.star LE le le' ->
-    T.star TE te te' ->
-    L.value le' ->
-    T.value te' ->
-    match_states LE TE le te ->
-    match_states LE TE le' te'.
-Admitted.
-
-
-
-
-
-
-Definition Pred := L.expr -> T.expr -> Prop.
-
-(* rel n : Pred *)
-(* later n : {m | m < n} -> Pred *)
-(* later n m = rel m *)
-
-
-Inductive L_callable : L.expr -> Prop :=
-| LCallable : forall fname free, L_callable (L.Close fname free).
-
-Inductive T_callable : T.expr -> Prop :=
-| TCallable : forall fname free, T_callable (T.Close fname free).
-
-Inductive rel' (LE : L.env) (TE : T.env) (n : nat)
-    (later : forall m, m < n -> Pred) : Pred :=
-| RelData : forall c largs targs,
-        Forall2 (rel' LE TE n later) largs targs ->
-        rel' LE TE n later
-            (L.Constr c largs)
-            (T.Constr (Utopia.constructor_index c) targs)
-| RelFunc : forall lf tf,
-        L_callable lf ->
-        T_callable tf ->
-        (forall m Hlt la ta lr tr,
-            L.value la -> T.value ta ->
-            L.value lr -> T.value tr ->
-            L.star LE (L.Call lf la) lr ->
-            T.star TE (T.Call tf ta) tr ->
-            (later m Hlt) la ta ->
-            (later m Hlt) lr tr) ->
-        rel' LE TE n later lf tf
-.
-
-Fixpoint rel5 (LE : L.env) (TE : T.env) x : forall y, y < x -> Pred :=
-    fun y Hy =>
-        let later : forall z, z < y -> Pred :=
-            fun z Hz =>
-                match x as x_ return y < x_ -> Pred with
-                | 0 => fun _ _ _ => True
-                | S x => fun Hy =>
-                        rel5 LE TE x z ltac:(hide; omega)
-                end Hy
-        in rel' LE TE y later.
-
-Definition rel50 (LE : L.env) (TE : T.env) x : Pred :=
-    rel' LE TE x (rel5 LE TE x).
-
-
-
-
-
-Lemma rel'_rel' : forall LE TE n later1 later2,
-    (forall m Hm le te, later1 m Hm le te <-> later2 m Hm le te) ->
-    forall le te,
-    rel' LE TE n later1 le te ->
-    rel' LE TE n later2 le te.
-intros0 Hlater.
-induction le using L.expr_ind'; intros0 Hrel;
-invc Hrel;
-try on (L_callable _), invc;
-try on (T_callable _), invc.
-
-- constructor.
-  assert (forall i,
-    forall le, nth_error args i = Some le ->
-    forall te, nth_error targs i = Some te ->
-    (forall te,
-        rel' LE TE n later1 le te ->
-        rel' LE TE n later2 le te) ->
-    rel' LE TE n later1 le te ->
-    rel' LE TE n later2 le te) by (intros; eauto).
-  list_magic **.
-
-- constructor; try constructor.  intros.
-  rename H2 into HH.
-  specialize (HH ?? ** la ta lr tr ** ** ** ** ** **).
-  rewrite Hlater, Hlater in HH.
-  eauto.
-Qed.
-
-Lemma rel'_rel'_iff : forall LE TE n later1 later2,
-    (forall m Hm le te, later1 m Hm le te <-> later2 m Hm le te) ->
-    forall le te,
-    rel' LE TE n later1 le te <-> rel' LE TE n later2 le te.
-intros; split; eapply rel'_rel'.
-- eauto.
-- intros. split; intro; [rewrite H | rewrite <- H]; eauto.
-Qed.
-
-
-Lemma rel5_irrel : forall LE TE x y Hy1 Hy2 le te,
-    rel5 LE TE x y Hy1 le te <-> rel5 LE TE x y Hy2 le te.
-induction x; intros; try omega.
-simpl. eapply rel'_rel'_iff. intros.
-eapply IHx.
-Qed.
-
-Lemma rel5_rel5 : forall LE TE x1 x2 y Hy1 Hy2 le te,
-    rel5 LE TE x1 y Hy1 le te <-> rel5 LE TE x2 y Hy2 le te.
-induction x1; induction x2; intros; try omega.
-
-simpl. eapply rel'_rel'_iff. intros.
-eapply IHx1.
-Qed.
-
-Lemma rel5_50 : forall LE TE x y Hlt,
-    (forall le te, rel5 LE TE x y Hlt le te <-> rel50 LE TE y le te).
-induction x; intros; try omega.
-
-unfold rel50; simpl.
-eapply rel'_rel'_iff. intros.
-eapply rel5_rel5.
-Qed.
-
-Lemma rel'_pred : forall LE TE x later1 later2,
-    (forall y Hy1 Hy2 le te,
-        later1 y Hy1 le te <-> later2 y Hy2 le te) ->
-    forall le te,
-    rel' LE TE (S x) later1 le te ->
-    rel' LE TE x later2 le te.
-intros0 Hlater.
-induction le using L.expr_ind';
-intros0 Hrel; invc Hrel;
-try on (L_callable _), invc;
-try on (T_callable _), invc.
-
-- constructor.
-  assert (forall i,
-    forall le, nth_error args i = Some le ->
-    forall te, nth_error targs i = Some te ->
-    (forall te,
-        rel' LE TE (S x) later1 le te ->
-        rel' LE TE x later2 le te) ->
-    rel' LE TE (S x) later1 le te ->
-    rel' LE TE x later2 le te) by (intros; eauto).
-  list_magic **.
-
-- constructor; try constructor.  intros.
-  rename H2 into HH.
-  specialize (HH m ltac:(hide; omega) la ta lr tr ** ** ** ** ** **).
-  rewrite Hlater, Hlater in HH.
-  eauto.
-Qed.
-
-Lemma rel50_pred : forall LE TE x,
-    forall le te,
-    rel50 LE TE (S x) le te ->
-    rel50 LE TE x le te.
-unfold rel50. intros0 Hrel.
-eapply rel'_pred; eauto. intros.
-eapply rel5_rel5.
-Qed.
-
-
-
-
-
-
-
-Inductive match_states2' (LE : L.env) (TE : T.env) (n : nat)
-    (later : forall m, m < n -> Pred) : Pred :=
-| Ms2Arg :
-        match_states2' LE TE n later L.Arg T.Arg
-| Ms2UpVar : forall i,
-        match_states2' LE TE n later (L.UpVar i) (T.UpVar i)
-| Ms2Call : forall lf la tf ta,
-        match_states2' LE TE n later lf tf ->
-        match_states2' LE TE n later la ta ->
-        match_states2' LE TE n later (L.Call lf la) (T.Call tf ta)
-| Ms2Constr : forall c largs tag targs,
-        Utopia.constructor_index c = tag ->
-        Forall2 (match_states2' LE TE n later) largs targs ->
-        match_states2' LE TE n later (L.Constr c largs) (T.Constr tag targs)
-| Ms2Elim : forall ty lcases ltarget tcases0 tcases ttarget,
-        Forall2 (match_states2' LE TE n later) lcases tcases0 ->
-        mk_tagged_cases ty tcases0 = Some tcases ->
-        match_states2' LE TE n later ltarget ttarget ->
-        match_states2' LE TE n later (L.Elim ty lcases ltarget) (T.Elim tcases ttarget)
-| Ms2Close : forall fn largs targs,
-        Forall2 (match_states2' LE TE n later) largs targs ->
-        match_states2' LE TE n later (L.Close fn largs) (T.Close fn targs)
-
-| Ms2FExt : forall lfn lfree tfn tfree,
-        Forall L.value lfree ->
-        Forall T.value tfree ->
-        (forall m Hlt la ta lr tr,
-            L.value la -> T.value ta ->
-            L.value lr -> T.value tr ->
-            L.star LE (L.Call (L.Close lfn lfree) la) lr ->
-            T.star TE (T.Call (T.Close tfn tfree) ta) tr ->
-            (later m Hlt) la ta ->
-            (later m Hlt) lr tr) ->
-        match_states2' LE TE n later (L.Close lfn lfree) (T.Close tfn tfree)
-.
-
-Fixpoint match_states2_later (LE : L.env) (TE : T.env) x : forall y, y < x -> Pred :=
-    fun y Hy =>
-        let later : forall z, z < y -> Pred :=
-            fun z Hz =>
-                match x as x_ return y < x_ -> Pred with
-                | 0 => fun _ _ _ => True
-                | S x => fun Hy =>
-                        match_states2_later LE TE x z ltac:(hide; omega)
-                end Hy
-        in match_states2' LE TE y later.
-
-Definition match_states2 (LE : L.env) (TE : T.env) x : Pred :=
-    match_states2' LE TE x (match_states2_later LE TE x).
-
-
-Theorem match2_value_LT : forall LE TE n le te,
-    match_states2 LE TE n le te ->
-    L.value le ->
-    T.value te.
-induction le using L.expr_ind'; intros0 Hmatch Lval; invc Lval; invc Hmatch; constructor;
-fold (match_states2 LE TE n) in *.
-
-- assert (forall i,
-    forall le, nth_error args i = Some le ->
-    forall te, nth_error targs i = Some te ->
-    (forall te, match_states2 LE TE n le te -> L.value le -> T.value te) ->
-    match_states2 LE TE n le te ->
-    L.value le ->
-    T.value te) by eauto.
-  list_magic **.
-
-- assert (forall i,
-    forall le, nth_error free i = Some le ->
-    forall te, nth_error targs i = Some te ->
-    (forall te, match_states2 LE TE n le te -> L.value le -> T.value te) ->
-    match_states2 LE TE n le te ->
-    L.value le ->
-    T.value te) by eauto.
-  list_magic **.
-
-- assumption.
-Qed.
-
-Theorem match2_value_TL : forall LE TE n te le,
-    match_states2 LE TE n le te ->
-    T.value te ->
-    L.value le.
-Admitted.    (* missing T.expr_ind' *)
-
-
-Theorem L_value_cant_step : forall LE le le',
-    L.value le ->
-    L.step LE le le' ->
-    False.
-induction le using L.expr_ind'; intros0 Hval Hstep; invc Hval; invc Hstep.
-
-- rewrite Forall_forall in *.
-  assert (In e (vs ++ e :: es)). { eapply in_or_app. right. left. reflexivity. }
-  eauto.
-
-- rewrite Forall_forall in *.
-  assert (In e (vs ++ e :: es)). { eapply in_or_app. right. left. reflexivity. }
-  eauto.
-Qed.
-
-Theorem T_value_cant_step : forall TE te te',
-    T.value te ->
-    T.step TE te te' ->
-    False.
-Admitted.    (* missing T.expr_ind' *)
-
-
-    (*
-Theorem match2_step : forall LE TE n le le' te te',
-    Forall2 (match_states2 LE TE n) LE TE ->
-    match_states2 LE TE n le te ->
-    L.step LE le le' ->
-    T.step TE te te' ->
-    match_states2 LE TE n le' te'.
-intros. move le at top. generalize_all.
-induction le using L.expr_ind'; intros0 Henv Hmatch Lstep Tstep;
-try solve [invc Lstep]; invc Hmatch.
-
-- (* Call *)
-  inv Lstep.
-
-  + (* MakeCall *)
-    inv Tstep.
-    Focus 2. fwd eapply match2_value_LT; eauto using L.VClose.
-      exfalso. eauto using T_value_cant_step.
-    Focus 2. assert (T.value ta) by (eauto using match2_value_LT).
-      exfalso. eauto using T_value_cant_step.
-
-    invc H1.
-    -- (* Ms2Close - arg + free match, same fname *)
-       admit. (* need substitution lemma *)
-    -- 
-
-  +  
-
-  + (* MakeCall *)
-    invc Hmatch. invc H4.
-
-    eexists. split.
-    -- fwd eapply Forall2_nth_error_Some with (xs := LE) (ys := TE); eauto.  break_exists.
-       eapply T.MakeCall; eauto using match_value.
-
-       ++ assert (forall i,
-            forall lv, nth_error free i = Some lv ->
-            forall tv, nth_error targs i = Some tv ->
-            match_states LE TE lv tv ->
-            L.value lv ->
-            T.value tv) by (eauto using match_value).
-          list_magic **.
-
-       ++ admit. (* T.subst succeeds because L.subst succeeds *)
-
-    -- admit. (* (1) needs subst/match lemma; (2) need to know how te' was made *)
-
-  + (* CallL *)
-    invc Hmatch.
-    fwd eapply IHle1; eauto. 
-    break_exists. break_and.
-    eexists. split; econstructor; eauto.
-
-  + (* CallR *)
-    invc Hmatch.
-    fwd eapply IHle2; eauto.
-    break_exists. break_and.
-    eexists. split; econstructor; solve [eauto using match_value].
-
-- (* Constr *)
-  invc Lstep. invc Hmatch.
-  admit.
-
-- admit.
-- admit.
-Admitted.
-*)
-
-
-
-
-
-(* Can't really see any way to prove this, which seems bad...
-
-Theorem match_states_rel50 : forall LE TE le te,
-    Forall2 (match_states LE TE) LE TE ->
-    L.value le ->
-    T.value te ->
-    match_states LE TE le te <-> (forall n, rel50 LE TE n le te).
-(* party time! *)
-induction le using L.expr_ind'; try rename H into IHle;
-intros0 Henv Lval Tval; try solve [invc Lval];
-split; intro Hmatch.
-
-- (* Constr *)
-  invc Hmatch. invc Lval. invc Tval.
-  constructor.
-  change (rel' _ _ _ _) with (rel LE TE n).
-
-  assert (HH : forall i,
-    forall arg, nth_error args i = Some arg ->
-    forall targ, nth_error targs i = Some targ ->
-    (fun le => forall te,
-        match_states LE TE le te ->
-        L.value le -> T.value te ->
-        rel LE TE n le te) arg ->
-    L.value arg ->
-    T.value targ ->
-    match_states LE TE arg targ ->
-    rel LE TE n arg targ) by eauto.
-
-  list_magic **.
-
-- (* Close *)
-  inv Hmatch. inv Lval. inv Tval.
-  constructor. intros.
-
-  fwd eapply match_star_value; eauto.
-    (* uh oh *) admit.
-  fwd eapply IHn as Hrel; eauto.
-    (* ??? *)
-Admitted.
-
-*)
-
-
-
-
-
-
-
-(* bunch of broken/useless stuff
-
-
-
-
-Definition rel (LE : L.env) (TE : T.env) (n : nat) : Pred.
-induction n using (Fix lt_wf).
-eapply rel'; try eassumption.
-Defined.
-
-
-Definition Fix_lt P F x :=
-    @Fix_F nat lt P F x (lt_wf x).
-
-Check Fix_lt.
-
-
-Fixpoint Fix_lt'
-    (P : nat -> Type)
-    (F : forall x, (forall y, y < x -> P y) -> P x)
-    (x : nat) {struct x} : forall y, y < x -> P y.
-intros. specialize (Fix_lt' P F).
-destruct x.
-- hide; omega.
-- specialize (Fix_lt' x).
-  destruct (eq_nat_dec x y).
-  + rewrite <- e. eapply F. assumption.
-  + eapply Fix_lt'. hide; omega.
-Defined.
-
-Definition Fix_lt'' 
-    (P : nat -> Type)
-    (F : forall x, (forall y, y < x -> P y) -> P x)
-    (x : nat) : P x.
-simple refine (
-    let fix go (n : nat) {struct n} : forall (m : nat), m < n -> P m := _ in
-    F x (go x)
-).
-
-destruct n; intros.
-- hide; omega.
-- destruct (eq_nat_dec m n) as [Heq | Hne].
-  + rewrite Heq. eapply F. eapply go.
-  + eapply (go n). hide; omega.
-Defined.
-
-Definition Fix_lt'''
-    (P : nat -> Type)
-    (F : forall x, (forall y, y < x -> P y) -> P x) :
-    forall x, forall y, y < x -> P y.
-fix 1.
-intros. eapply F.
-destruct x. { hide. exfalso. omega. }
-specialize (Fix_lt''' x).
-
-destruct (eq_nat_dec y x) as [Heq | Hne].
-- rewrite Heq. eapply Fix_lt'''.
-- intros. eapply Fix_lt'''. hide. omega.
-Defined.
-
-Print Fix_lt'''.
-
-Definition rel3 (LE : L.env) (TE : T.env) : forall x, forall y, y < x -> Pred.
-fix 1.
-destruct x; intros.
-{ hide. omega. }
-
-eapply (rel' LE TE x). eauto.
-Defined.
-Print rel3.
-
-Fixpoint rel4 (LE : L.env) (TE : T.env) x : forall y, y < x -> Pred :=
-    match x as x_ return forall y, y < x_ -> Pred with
-    | 0 => fun _ _ _ _ => True
-    | S x => fun y Hy =>
-        let later : forall z, z < y -> Pred :=
-            fun z Hz => rel4 LE TE x z ltac:(hide; omega) in
-        rel' LE TE y later
-    end.
-
-Print rel4.
-
-Definition rel40 (LE : L.env) (TE : T.env) x : Pred :=
-    rel' LE TE x (rel4 LE TE x).
-
-
-
-
-
-
-Definition nat_ind_strong'
-    (P : nat -> Prop)
-    (HO : P 0)
-    (HS : forall n, (forall m, m <= n -> P m) -> P (S n))
-    (n : nat) : forall m, m <= n -> P m.
-induction n; intros0 Hlt.
-- assert (m = 0) by (hide; omega). subst. assumption.
-- inversion Hlt.
-  + eapply HS. eauto.
-  + eapply IHn. eauto.
-Defined.
-
-Definition nat_ind_strong'2
-    (P : nat -> Type)
-    (HO : P 0)
-    (HS : forall n, (forall m, m <= n -> P m) -> P (S n))
-    (n : nat) : forall m, m <= n -> P m.
-induction n; intros0 Hlt.
-- assert (m = 0) by (hide; omega). subst. assumption.
-- destruct (eq_nat_dec m (S n)).
-  + subst m. eapply HS. assumption.
-  + assert (m <= n) by (hide; omega). eapply IHn. assumption.
-Defined.
-
-Definition nat_ind_strong'3
-    (P : nat -> Type)
-    (Acc : forall n, (forall m, m < n -> P m) -> P n)
-    (n : nat) : forall m, m < n -> P m.
-induction n; intros0 Hlt.
-- exfalso. hide. omega.
-- destruct (eq_nat_dec m n).
-  + subst m. eapply Acc. assumption.
-  + assert (m < n) by (hide; omega). eapply IHn. assumption.
-Defined.
-
-Definition nat_ind_strong'4
-    (P : nat -> Type)
-    (HO : P 0)
-    (HS : forall n, P n -> P (S n))
-    (n : nat) : forall m, m <= n -> P m.
-induction n; intros0 Hlt.
-- assert (m = 0) by (hide; omega). subst. assumption.
-- destruct (eq_nat_dec m (S n)).
-  + subst m. eapply HS. eapply IHn. hide; omega.
-  + assert (m <= n) by (hide; omega). eapply IHn. assumption.
-Defined.
-
-Definition nat_ind_strong'5
-    (P : nat -> Type)
-    (HO : P 0)
-    (HS : forall n, P n -> P (S n))
-    (n : nat) : forall m, m < n -> P m.
-induction n; intros0 Hlt.
-- hide; omega.
-- destruct (eq_nat_dec m n).
-  + subst m. destruct n; eauto.
-  + assert (m < n) by (hide; omega). eapply IHn. assumption.
-Defined.
-
-Definition nat_ind_strong
-    (P : nat -> Type)
-    (Acc : forall n, (forall m, m < n -> P m) -> P n)
-    (n : nat) : P n.
-eapply Acc. eapply nat_ind_strong'3. assumption.
-Defined.
-
-
-(* srel n x y = forall m, m < n -> rel m x y *)
-(* rel n x y = rel' (srel n) x y *)
-
-Inductive strong {A B} (R : nat -> A -> B -> Prop) : nat -> A -> B -> Prop :=
-| StrongZero : forall a b, strong R 0 a b
-| StrongSucc : forall n a b,
-        R n a b ->
-        strong R n a b ->
-        strong R (S n) a b.
-
-Lemma strong_forall : forall A B (R : nat -> A -> B -> Prop) n a b,
-    strong R n a b ->
-    forall m, m < n -> R m a b.
-induction n; intros0 Hstrong; intros0 Hlt.
-{ invc Hlt. }
-invc Hstrong. destruct (eq_nat_dec m n).
-- subst. assumption.
-- eapply IHn; eauto. omega.
-Qed.
-
-Lemma forall_strong : forall A B (R : nat -> A -> B -> Prop) n a b,
-    (forall m, m < n -> R m a b) ->
-    strong R n a b.
-induction n; intros0 Hr.
-{ constructor. }
-constructor.
-- eauto.
-- eapply IHn. intros. eapply Hr. omega.
-Qed.
-
-Lemma strong_forall_iff : forall A B (R : nat -> A -> B -> Prop) n a b,
-    strong R n a b <-> (forall m, m < n -> R m a b).
-intros. split.
-- eapply strong_forall.
-- eapply forall_strong.
-Qed.
-
-
-
-
-
-
-Lemma rel5_pred : forall LE TE x le te,
-    x > 0 ->
-    rel50 LE TE x le te ->
-    rel50 LE TE (pred x) le te.
-induction x; intros0 Hgt Hrel; try omega.
-
-unfold rel50 in *; simpl in *.
-
-Focus 2.
-
-- unfold rel50 in *. invc Hrel.
-  constructor.
-unfold rel50.
-
-
-
-
-Fixpoint rel4 (LE : L.env) (TE : T.env) x : forall y, y < x -> Pred.
-refine (fun y Hy => rel' LE TE x _).
-    rel' LE TE x 
-    match x as x_ return forall y, y < x_ -> Pred with
-    | 0 => fun y Hy => ltac:(hide; exfalso; omega)
-    | S x => fun y Hy => rel' LE TE x (rel4 LE TE x)
-    end.
-
-destruct (eq_nat_dec y x) as [Heq | Hne].
-- eapply (rel' LE TE x).
-
-intros. eapply (rel' LE TE x).
-destruct x eqn:?. { hide. exfalso. omega. }
-specialize (rel3 n).
-
-destruct (eq_nat_dec y n) as [Heq | Hne].
-- rewrite <- Heqn. eapply (rel
-- intros. eapply Fix_lt'''. hide. omega.
-Defined.
-
-
-Definition Fix_lt'4
-    (P : nat -> Type)
-    (F : forall x, (forall y, y < x -> P y) -> P x) :
-    forall x, forall y, y < x -> P y.
-fix 1.
-intros. eapply F.
-destruct (eq_nat_dec (S y) x) as [Heq | Hne].
-- intros. eapply F.
-rewrite Heq. eapply Fix_lt'4.
-- intros. eapply Fix_lt'4. hide. omega.
-Defined.
-
-Print Fix_lt'4.
-
-
-
-- eapply (go n). hide; omega.
-
-- omega.
-
-simple refine (
-    
-
-
-
-
-Fixpoint Fix_lt''
-    (P : nat -> Type)
-    (F : forall x, (forall y, y < x -> P y) -> P x)
-    (x : nat) {struct x} : forall y, y < x -> P y.
-
-intros. specialize (Fix_lt' P F).
-destruct x.
-- omega.
-- specialize (Fix_lt' x).
-  destruct (eq_nat_dec x y).
-  + subst y. eapply F. assumption.
-  + eapply Fix_lt'. omega.
-Defined.
-
-Definition rel2 (LE : L.env) (TE : T.env) (n : nat) : Pred.
-refine (let fix go n m Hlt := rel' LE TE n 
-generalize n. clear n. fix 1. intro n.
-
-
-  + eapply F.
-
-
-
-
-refine (F x (fun y Hlt => _)).
-
-generalize dependent x. fix 1.
-intros. dest
-- hide; omega.
-- destruct (eq_nat_dec x y) as [Heq | Hne].
-  + rewrite <- Heq. eapply Fix_lt'. exact F.
-  + 
-induction y.
-- eapply F. intros. exfalso; hide; omega.
-- eapply F.
-
-
-
-Definition rel (LE : L.env) (TE : T.env) (n : nat) : Pred.
-induction n using Fix_lt.
-eapply rel'; try eassumption.
-Defined.
-
-Print rel.
-
-
-Lemma Fix_lt_eq :
-    forall P F x,
-    F x (fun (y : nat) (Hlt : y < x) => Fix_lt P F y) = Fix_lt P F x.
-intros. unfold Fix_lt. rewrite <- Fix_F_eq.
-f_equal. unfold lt_wf, well_founded_ltof.
-
-
-Lemma Fix_F_eq :
-    forall (x:A) (r:Acc x),
-    F (fun (y:A) (p:R y x) => Fix_F (x:=y) (Acc_inv r p)) = Fix_F (x:=x) r.
-
-Check Fix_eq.
-
-(*
-Definition later (LE : L.env) (TE : T.env) n : forall m, m < n -> Pred.
-induction n using (Fix lt_wf).
-intros m Hlt.
-eapply rel'; try eassumption.
-specialize (X ?? Hlt).
-eassumption.
-Defined.
-
-Eval cbv beta delta[later] in later.
-Eval cbv beta delta[rel] in rel.
-*)
-
-
-Lemma rel_pred : forall LE TE n le te,
-    rel LE TE (S n) le te ->
-    rel LE TE n le te.
-induction n; intros0 Hrel.
-- unfold rel in *.
-
-
-
-
-Definition rel LE TE n := nat_ind_strong _ (rel' LE TE) n.
-
-(*
-Inductive rel' (LE : L.env) (TE : T.env) :
-    forall (n : nat) (strong : forall m, m < n -> L.expr -> T.expr -> Prop),
-    L.expr -> T.expr -> Prop :=
-| RelData : forall n strong c largs targs,
-        Forall2 (rel' LE TE n strong) largs targs ->
-        rel' LE TE n strong
-            (L.Constr c largs)
-            (T.Constr (Utopia.constructor_index c) targs)
-| RelFunc : forall n (strong : forall m, _ -> _ -> _ -> Prop) lf tf,
-        (forall la ta lr tr m (Hlt : m < n),
-            L.value la -> T.value ta ->
-            L.value lr -> T.value tr ->
-            L.star LE (L.Call lf la) lr ->
-            T.star TE (T.Call tf ta) tr ->
-            strong m Hlt la ta ->
-            strong m Hlt lr tr) ->
-        rel' LE TE n strong lf tf
-.
-
-Definition rel LE TE n := nat_ind_strong _ (rel' LE TE) n.
-*)
-
-(* The base case has magically disappeared.  Now all functions are rel at level
- * 0 because there are no `m < 0`. *)
-
-
-
-
-Theorem match_states_rel : forall LE TE le te,
-    Forall2 (match_states LE TE) LE TE ->
-    L.value le ->
-    T.value te ->
-    match_states LE TE le te <-> (forall n, rel LE TE n le te).
-(* party time! *)
-induction n using nat_ind_strong; rename H into IHn;
-induction le using L.expr_ind'; try rename H into IHle;
-intros0 Henv Hmatch Lval Tval; try solve [invc Lval].
-
-- (* Constr *)
-  invc Hmatch. invc Lval. invc Tval.
-  constructor.
-  change (rel' _ _ _ _) with (rel LE TE n).
-
-  assert (HH : forall i,
-    forall arg, nth_error args i = Some arg ->
-    forall targ, nth_error targs i = Some targ ->
-    (fun le => forall te,
-        match_states LE TE le te ->
-        L.value le -> T.value te ->
-        rel LE TE n le te) arg ->
-    L.value arg ->
-    T.value targ ->
-    match_states LE TE arg targ ->
-    rel LE TE n arg targ) by eauto.
-
-  list_magic **.
-
-- (* Close *)
-  inv Hmatch. inv Lval. inv Tval.
-  constructor. intros.
-
-  fwd eapply match_star_value; eauto.
-    (* uh oh *) admit.
-  fwd eapply IHn as Hrel; eauto.
-    (* ??? *)
-Admitted.
-
-*)
-
-
-
-Definition T_rename_globals (rename : nat -> nat) : T.expr -> T.expr :=
-    let fix go e :=
-        let fix go_list es :=
-            match es with
-            | [] => []
-            | e :: es => go e :: go_list es
-            end in
-        let fix go_cases cs :=
-            match cs with
-            | [] => []
-            | (e, r) :: cs => (go e, r) :: go_cases cs
-            end in
-        match e with
-        | T.Arg => T.Arg
-        | T.UpVar i => T.UpVar i
-        | T.Call f a => T.Call (go f) (go a)
-        | T.Constr tag args => T.Constr tag (go_list args)
-        | T.Elim cases target => T.Elim (go_cases cases) (go target)
-        | T.Close fname free => T.Close (rename fname) (go_list free)
-        end in go.
-
-Definition T_rename_globals_list (rename : nat -> nat) :=
-    let go := T_rename_globals rename in
-    let fix go_list es :=
-        match es with
-        | [] => []
-        | e :: es => go e :: go_list es
-        end in go_list.
-
-Definition T_rename_globals_cases (rename : nat -> nat) :=
-    let go := T_rename_globals rename in
-    let fix go_cases cs : list (T.expr * T.rec_info) :=
-        match cs with
-        | [] => []
-        | (e, r) :: cs => (go e, r) :: go_cases cs
-        end in go_cases.
-
-Inductive T_prog_equiv (E1 E2 : T.env) : (nat -> nat) -> T.expr -> T.expr -> Prop :=
-| TProgEquiv : forall rename e1 e2,
-        (forall fname code,
-            nth_error E1 fname = Some code ->
-            (* Looking up the renamed fname gives the renamed function *)
-            nth_error E2 (rename fname) = Some (T_rename_globals rename code)) ->
-        T_rename_globals rename e1 = e2 ->
-        T_prog_equiv E1 E2 rename e1 e2.
-
-
-
-Lemma T_rename_globals_list_app : forall rename es1 es2,
-    T_rename_globals_list rename (es1 ++ es2) =
-    T_rename_globals_list rename es1 ++ T_rename_globals_list rename es2.
-induction es1; intros; simpl.
-- reflexivity.
-- rewrite IHes1. reflexivity.
-Qed.
-
-Lemma T_rename_globals_list_cons : forall rename e es,
-    T_rename_globals_list rename (e :: es) =
-    T_rename_globals rename e :: T_rename_globals_list rename es.
-intros. simpl. reflexivity.
-Qed.
-
-Lemma T_rename_globals_list_map : forall rename es,
-    T_rename_globals_list rename es = map (T_rename_globals rename) es.
-induction es; simpl; eauto.
-Qed.
-
-Lemma T_rename_globals_list_length : forall rename es,
-    length (T_rename_globals_list rename es) = length es.
-intros. rewrite T_rename_globals_list_map. eapply map_length.
-Qed.
-
-Lemma Forall_map : forall A B (P : B -> Prop) (f : A -> B) xs,
-    Forall (fun x => P (f x)) xs ->
-    Forall P (map f xs).
-induction xs; intros.
-- constructor.
-- on (Forall _ _), invc. constructor; eauto.
-Qed.
-
-Lemma Forall_map_rev : forall A B (P : B -> Prop) (f : A -> B) xs,
-    Forall P (map f xs) ->
-    Forall (fun x => P (f x)) xs.
-induction xs; intros.
-- constructor.
-- on (Forall _ _), invc. constructor; eauto.
-Qed.
-
-Lemma app_inv_length : forall A (xs1 xs2 ys1 ys2 : list A),
-    length xs1 = length ys1 ->
-    xs1 ++ xs2 = ys1 ++ ys2 ->
-    xs1 = ys1 /\ xs2 = ys2.
-induction xs1; intros0 Hlen Happ; destruct ys1; simpl in *; try discriminate.
-- split; eauto.
-- invc Happ. invc Hlen. destruct (IHxs1 ?? ?? ?? ** **). subst. eauto.
-Qed.
-
-Lemma T_rename_globals_value : forall rename e,
-    T.value e ->
-    T.value (T_rename_globals rename e).
-induction e using T.expr_ind''; inversion 1; subst.
-
-- simpl. fold (T_rename_globals_list rename).
-  rewrite T_rename_globals_list_map.
-  constructor.
-
-  assert (forall i,
-    forall arg, nth_error args i = Some arg ->
-    (T.value arg -> T.value (T_rename_globals rename arg)) ->
-    T.value arg ->
-    T.value (T_rename_globals rename arg)) by (intros; eauto).
-  eapply Forall_map.
-  list_magic **.
-
-- simpl. fold (T_rename_globals_list rename).
-  rewrite T_rename_globals_list_map.
-  constructor.
-
-  assert (forall i,
-    forall val, nth_error free i = Some val ->
-    (T.value val -> T.value (T_rename_globals rename val)) ->
-    T.value val ->
-    T.value (T_rename_globals rename val)) by (intros; eauto).
-  eapply Forall_map.
-  list_magic **.
-
-Qed.
-
-Lemma T_rename_globals_list_value : forall rename es,
-    Forall T.value es ->
-    Forall T.value (T_rename_globals_list rename es).
-intros.
-rewrite T_rename_globals_list_map. eapply Forall_map.
-
-assert (forall i,
-    forall e, nth_error es i = Some e ->
-    T.value e ->
-    T.value (T_rename_globals rename e))
-    by (intros; eauto using T_rename_globals_value).
-list_magic **.
-Qed.
-
-Lemma T_rename_globals_value_rev : forall rename e,
-    T.value (T_rename_globals rename e) ->
-    T.value e.
-induction e using T.expr_ind''; inversion 1; subst.
-
-- simpl. fold (T_rename_globals_list rename) in *.
-  rewrite T_rename_globals_list_map in *.
-  constructor.
-
-  assert (forall i,
-    forall arg, nth_error args i = Some arg ->
-    (T.value (T_rename_globals rename arg) -> T.value arg) ->
-    T.value (T_rename_globals rename arg) ->
-    T.value arg) by (intros; eauto).
-  on _, fun H => eapply Forall_map_rev in H.
-  list_magic **.
-
-- simpl. fold (T_rename_globals_list rename) in *.
-  rewrite T_rename_globals_list_map in *.
-  constructor.
-
-  assert (forall i,
-    forall arg, nth_error free i = Some arg ->
-    (T.value (T_rename_globals rename arg) -> T.value arg) ->
-    T.value (T_rename_globals rename arg) ->
-    T.value arg) by (intros; eauto).
-  on _, fun H => eapply Forall_map_rev in H.
-  list_magic **.
-
-Qed.
-
-Lemma T_rename_globals_value_iff : forall rename e,
-    T.value (T_rename_globals rename e) <-> T.value e.
-intros; split; eauto using T_rename_globals_value, T_rename_globals_value_rev.
-Qed.
-
-Lemma leftmost_step_length : forall A (P : A -> Prop) vs1 e1 es1 vs2 e2 es2,
-    vs1 ++ [e1] ++ es1 = vs2 ++ [e2] ++ es2 ->
-    Forall P vs1 ->
-    ~P e1 ->
-    Forall P vs2 ->
-    ~P e2 ->
-    length vs1 = length vs2.
-induction vs1; intros0 Heq Hyes1 Hno1 Hyes2 Hno2; destruct vs2; simpl in *.
-
-- reflexivity.
-- invc Heq. invc Hyes2. exfalso. eauto.
-- invc Heq. invc Hyes1. exfalso. eauto.
-- invc Heq. invc Hyes1. invc Hyes2.
-  f_equal. eapply IHvs1; eauto.
-Qed.
-
-Lemma Forall_app_inv : forall A (P : A -> Prop) xs ys,
-    Forall P (xs ++ ys) ->
-    Forall P xs /\ Forall P ys.
-induction xs; intros; simpl in *.
-- eauto.
-- invc H. destruct (IHxs ?? **). eauto.
-Qed.
-
-Lemma map_Forall2 : forall A B (f : A -> B) xs ys,
-    Forall2 (fun x y => f x = y) xs ys ->
-    map f xs = ys.
-induction xs; intros0 Hfa; destruct ys; invc Hfa; simpl in *; eauto.
-f_equal. eapply IHxs; eauto.
-Qed.
-
-Lemma TEqCall : forall E1 E2 rename f1 a1 f2 a2,
-    (forall fname code,
-        nth_error E1 fname = Some code ->
-        (* Looking up the renamed fname gives the renamed function *)
-        nth_error E2 (rename fname) = Some (T_rename_globals rename code)) ->
-    T_prog_equiv E1 E2 rename f1 f2 ->
-    T_prog_equiv E1 E2 rename a1 a2 ->
-    T_prog_equiv E1 E2 rename (T.Call f1 a1) (T.Call f2 a2).
-intros0 Henv Heq1 Heq2.
-constructor; eauto.
-simpl. f_equal.
-- invc Heq1. reflexivity.
-- invc Heq2. reflexivity.
-Qed.
-
-Lemma TEqConstr : forall E1 E2 rename tag args1 args2,
-    (forall fname code,
-        nth_error E1 fname = Some code ->
-        (* Looking up the renamed fname gives the renamed function *)
-        nth_error E2 (rename fname) = Some (T_rename_globals rename code)) ->
-    Forall2 (T_prog_equiv E1 E2 rename) args1 args2 ->
-    T_prog_equiv E1 E2 rename (T.Constr tag args1) (T.Constr tag args2).
-intros0 Henv Heq.
-constructor; eauto.
-simpl. fold (T_rename_globals_list rename). f_equal.
-rewrite T_rename_globals_list_map.
-eapply map_Forall2.
-
-assert (forall i,
-    forall arg1, nth_error args1 i = Some arg1 ->
-    forall arg2, nth_error args2 i = Some arg2 ->
-    T_prog_equiv E1 E2 rename arg1 arg2 ->
-    T_rename_globals rename arg1 = arg2). {
-  intros. on (T_prog_equiv _ _ _ _ _), invc. reflexivity.
-}
-list_magic **.
-Qed.
-
-Lemma TEqClose : forall E1 E2 rename fname1 fname2 free1 free2,
-    (forall fname code,
-        nth_error E1 fname = Some code ->
-        (* Looking up the renamed fname gives the renamed function *)
-        nth_error E2 (rename fname) = Some (T_rename_globals rename code)) ->
-    rename fname1 = fname2 ->
-    Forall2 (T_prog_equiv E1 E2 rename) free1 free2 ->
-    T_prog_equiv E1 E2 rename (T.Close fname1 free1) (T.Close fname2 free2).
-intros0 Henv Hfn Hfree.
-constructor; eauto.
-simpl. fold (T_rename_globals_list rename). f_equal; eauto.
-rewrite T_rename_globals_list_map.
-eapply map_Forall2.
-
-assert (forall i,
-    forall arg1, nth_error free1 i = Some arg1 ->
-    forall arg2, nth_error free2 i = Some arg2 ->
-    T_prog_equiv E1 E2 rename arg1 arg2 ->
-    T_rename_globals rename arg1 = arg2). {
-  intros. on (T_prog_equiv _ _ _ _ _), invc. reflexivity.
-}
-list_magic **.
-Qed.
-
-Derive Inversion test_inv with
-    (forall E tag vs e es e', T.step E (T.Constr tag (vs ++ [e] ++ es)) e') Sort Prop.
-Check test_inv.
-
-Lemma T_step_constr_inv :
-    forall E tag vs e es rhs
-        (P : _ -> _ -> _ -> _ -> _ -> _ -> Prop),
-    Forall T.value vs ->
-    ~T.value e ->
-    (T.step E (T.Constr tag (vs ++ e :: es)) rhs ->
-     forall e'',
-     T.step E e e'' ->
-     rhs = T.Constr tag (vs ++ e'' :: es) ->
-     P E tag vs e es (T.Constr tag (vs ++ [e''] ++ es))) ->
-    T.step E (T.Constr tag (vs ++ [e] ++ es)) rhs ->
-    P E tag vs e es rhs.
-intros0 Hvals Hstep; intros0 Hinv Htop.
-inversion Htop.
-
-assert (length vs0 = length vs) by
-  (eapply leftmost_step_length; simpl; eauto using T_value_cant_step).
-
-on (_ ++ _ = _ ++ _), fun H => (eapply app_inv_length in H0; eauto). break_and.
-on (_ :: _ = _ :: _), fun H => invc H.
-eapply Hinv; eauto.
-Qed.
-
-Lemma Forall2_app : forall A B (P : A -> B -> Prop) xs1 xs2 ys1 ys2,
-    Forall2 P xs1 ys1 ->
-    Forall2 P xs2 ys2 ->
-    Forall2 P (xs1 ++ xs2) (ys1 ++ ys2).
-induction xs1; inversion 1; intros; simpl in *; eauto.
-Qed.
-
-Lemma T_rename_globals_prog_equiv : forall E1 E2 rename e,
-    (forall fname code,
-        nth_error E1 fname = Some code ->
-        (* Looking up the renamed fname gives the renamed function *)
-        nth_error E2 (rename fname) = Some (T_rename_globals rename code)) ->
-    T_prog_equiv E1 E2 rename e (T_rename_globals rename e).
-induction e using T.expr_ind''; intros; simpl; constructor; eauto.
-Qed.
-
-Lemma T_rename_globals_list_prog_equiv : forall E1 E2 rename es,
-    (forall fname code,
-        nth_error E1 fname = Some code ->
-        (* Looking up the renamed fname gives the renamed function *)
-        nth_error E2 (rename fname) = Some (T_rename_globals rename code)) ->
-    Forall2 (T_prog_equiv E1 E2 rename) es (T_rename_globals_list rename es).
-induction es; intros; simpl.
-- constructor.
-- specialize (IHes **).
-  constructor; eauto using T_rename_globals_prog_equiv.
-Qed.
-
-Theorem T_prog_equiv_step : forall E1 E2 rename e1 e2 e1' e2',
-    T.step E1 e1 e1' ->
-    T.step E2 e2 e2' ->
-    T_prog_equiv E1 E2 rename e1 e2 ->
-    T_prog_equiv E1 E2 rename e1' e2'.
-induction e1 using T.expr_ind''; intros0 Hstep1 Hstep2 Hequiv;
-invc Hstep1; invc Hequiv;
-simpl in *;
-try fold (T_rename_globals_list rename) in *;
-try fold (T_rename_globals_cases rename) in *.
-
-- admit.
-
-- invc Hstep2.
-  { assert (T.value e1_1).
-      { rewrite <- T_rename_globals_value_iff, <- **. constructor. eauto. }
-    exfalso. eapply T_value_cant_step; eauto.  }
-  Focus 2. { rewrite T_rename_globals_value_iff in *.
-    exfalso. eauto using T_value_cant_step. } Unfocus.
-
-  eapply TEqCall; eauto using T_rename_globals_prog_equiv.
-
-- invc Hstep2.
-  { rewrite T_rename_globals_value_iff in *. exfalso. eauto using T_value_cant_step. }
-  { rewrite <- T_rename_globals_value_iff in *. exfalso. eauto using T_value_cant_step. }
-
-  eapply TEqCall; eauto using T_rename_globals_prog_equiv.
-
-- rewrite T_rename_globals_list_app, T_rename_globals_list_cons in Hstep2.
-  inversion Hstep2 using T_step_constr_inv; intros.
-    { eauto using T_rename_globals_list_value. }
-    { rewrite T_rename_globals_value_iff. eauto using T_value_cant_step. }
-  subst.  clear Hstep2 H1.
-
-  eapply TEqConstr; eauto.
-  eapply Forall2_app; [ | constructor ].
-
-  + eapply T_rename_globals_list_prog_equiv; eauto.
-
-  + on (Forall _ (_ ++ _)), fun H => eapply Forall_app_inv in H. break_and.
-    on (Forall _ (_ :: _)), invc.
-    eapply H7; eauto.
-    eapply T_rename_globals_prog_equiv; eauto.
-
-  + eapply T_rename_globals_list_prog_equiv; eauto.
-
-- admit.
-
-- admit.
-
-- admit.
-
-Admitted.
-
-
-Inductive rel (LE : L.env) (TE : T.env) : L.expr -> T.expr -> Prop :=
+Inductive R (LE : L.env) (TE : T.env) : L.expr -> T.expr -> Prop :=
 | RConstr : forall c largs targs,
-        Forall2 (rel LE TE) largs targs ->
-        rel LE TE
+        Forall2 (R LE TE) largs targs ->
+        R LE TE
             (L.Constr c largs)
             (T.Constr (Utopia.constructor_index c) targs)
-| RClose : forall rename lfn tfn lf tf TE' tf' lfree tfree,
-        nth_error LE lfn = Some lf ->
-        nth_error TE tfn = Some tf ->
-        compile_program (lf, LE) = Some (tf', TE') ->
-        T_prog_equiv TE TE' rename tf tf' ->
-        Forall2 (rel LE TE) lfree tfree ->
-        rel LE TE
-            (L.Close lfn lfree)
-            (T.Close tfn tfree)
+| RClose : forall fn lf tf lfree tfree,
+        nth_error LE fn = Some lf ->
+        nth_error TE fn = Some tf ->
+        compile_program (lf, LE) = Some (tf, TE) ->
+        Forall2 (R LE TE) lfree tfree ->
+        R LE TE
+            (L.Close fn lfree)
+            (T.Close fn tfree)
 .
 
-(*
-- rewrite T_rename_globals_list_app, T_rename_globals_list_cons in Hstep2.
-  assert (Forall T.value (T_rename_globals_list rename vs))
-    by (eauto using T_rename_globals_list_value).
-  invc Hstep2.
 
-  assert (length vs0 = length (T_rename_globals_list rename vs)). {
-    eapply leftmost_step_length; simpl; try eassumption.
-    - intro. eapply T_value_cant_step; eauto.
-    - rewrite T_rename_globals_value_iff.
-      intro. eapply T_value_cant_step; eauto.
-  }
-  fwd eapply app_inv_length; eauto. break_and.
-  on _, invc.
+(* inductive relation *)
 
-  econstructor; eauto. simpl. fold (T_rename_globals_list rename).
-  rewrite T_rename_globals_list_app, T_rename_globals_list_cons in *.
-  f_equal. f_equal; eauto. f_equal; eauto.
-
-  on (Forall _ (_ ++ _)), fun H => eapply Forall_app_inv in H. break_and.
-  on (Forall _ (_ :: _)), invc.
-  specialize ( H11 ?? ?? ?? ** ** ).
-*)
-
-
-(*
-  invc H1.
-
-  fwd simple refine (T_step_constr_inv vs e ** _); eauto using T_value_cant_step.
-  inversion Hstep2 using H1.
-  inversion Hstep2 using (T_step_constr_inv ?? vs e e' ** ** ).
-
-  fwd simple refine (fun rhs P => T_step_constr_inv ?? ?? ?? ?? ?? ?? rhs P ** ** ) as HH.
-  inversion Hstep2 using HH.
-
-invc Hstep2. eapply TEqConstr; eauto. simpl.
-  on (Forall _ (_ ++ _)), fun H => eapply Forall_app_inv in H. break_and.
-  on (Forall _ (_ :: _)), invc.
-    (eapply Forall_app_inv in H; destruct H as [? H]).
-
-
-
-
-  eapply Forall2_app; [ | constructor ].
-
-
-  assert (Forall T.value (T_rename_globals_list rename vs))
-    by (eauto using T_rename_globals_list_value).
-  invc Hstep2.
-  rewrite T_rename_globals_list_app, T_rename_globals_list_cons in *.
-
-  assert (length vs0 = length (T_rename_globals_list rename vs)). {
-    eapply leftmost_step_length; simpl; try eassumption.
-    - intro. eapply T_value_cant_step; eauto.
-    - rewrite T_rename_globals_value_iff.
-      intro. eapply T_value_cant_step; eauto.
-  }
-  fwd eapply app_inv_length; eauto. break_and.
-  on _, invc.
-
-  econstructor; eauto. simpl. fold (T_rename_globals_list rename).
-  rewrite T_rename_globals_list_app, T_rename_globals_list_cons in *.
-  f_equal. f_equal; eauto. f_equal; eauto.
-  SearchAbout (Forall _ (_ ++ _)).
-  fwd eapply Forall_app; eauto. break_and.
-  on (Forall _ (_ :: _)), invc.
-
-  specialize (H12 ?? ?? ?? ** ** ).
-  fwd eapply H12. { econstructor; eauto. }
-  invc H9. eauto.
-
-
-  on (Forall _ (_ ++ _)), invc.  { destruct vs; discriminate. }
-
-  assert (length vs = length vs0).
-
-  fwd eapply app_inv_length; try eassumption; eauto using T_rename_globals_list_length.
-  eapply app_inv_length in H3.
-  SearchAbout (_ ++ _ = _ ++ _ -> _).
-  congruence.
-
-        
-
-Inductive T_prog_equiv : T.env -> T.env -> T.expr -> T.expr :
-    exists f,
-        (forall i , nth_error E1 
-        T_rename_globals 
-
-
-Inductive T_prog_equiv (E1 E2 : T.env) : (nat -> nat) -> T.expr -> T.expr -> Prop :=
-| EqArg : T_prog_equiv E1 E2 T.Arg T.Arg
-| EqUpvar : forall i, T_prog_equiv E1 E2 (T.UpVar i) (T.UpVar i)
-| EqCall : forall f1 a1 f2 a2,
-        T_prog_equiv E1 E2 f1 f2 ->
-        T_prog_equiv E1 E2 a1 a2 ->
-        T_prog_equiv E1 E2 (T.Call f1 a1) (T.Call f2 a2)
-| EqConstr : forall tag args1 args2,
-        Forall2 (T_prog_equiv E1 E2) args1 args2 ->
-        T_prog_equiv E1 E2 (T.Constr tag args1) (T.Constr tag args2)
-| EqElim : forall cases1 cases2 target1 target2,
-        Forall2 (fun case1 case2 => T_prog_equip E1 E2 (fst case1) (fst case2)) cases1 cases2 ->
-        T_prog_equip E1 E2 target1 target2 ->
-        T_prog_equiv E1 E2 (T.Elim cases1 target1) (T.Elim cases2 target2)
-| EqClose
-
-.
-
-  *)
-
-
-Inductive match_states3 (LE : L.env) (TE : T.env) : L.expr -> T.expr -> Prop :=
-| MatchStates3 : forall le te,
+Inductive I (LE : L.env) (TE : T.env) : L.expr -> T.expr -> Prop :=
+| ICompile : forall l t,
         compile_list LE = Some TE ->
-        compile le = Some te ->
-        match_states3 LE TE le te.
+        compile l = Some t ->
+        I LE TE l t.
 
-Theorem compile_match_states3 : forall LE le TE te,
-    compile_program (le, LE) = Some (te, TE) ->
-    match_states3 LE TE le te.
-intros0 Hcomp.
-unfold compile_program in Hcomp.
-compute [seq fmap bind_option] in Hcomp. repeat (break_match; try discriminate).
-repeat (on (Some _ = Some _), invc). compute [fst snd] in *.
-on ((_, _) = (_, _)), invc.
-constructor; assumption.
+
+
+(* proofs *)
+
+Ltac refold_compile := fold compile_list in *.
+Ltac simpl_compile := simpl in *; refold_compile.
+
+Lemma Forall2_I_compile_list : forall LE TE ls ts,
+    Forall2 (I LE TE) ls ts ->
+    compile_list ls = Some ts.
+induction ls; intros0 Hfa; destruct ts; invc Hfa; simpl in *; eauto.
+unfold seq, fmap.
+specialize (IHls ?? **). rewrite IHls. simpl.
+on (I _ _ _ _), invc. rewrite **. simpl.
+reflexivity.
 Qed.
 
-Lemma compile_list_Forall2 : forall es es',
-    compile_list es = Some es' ->
-    Forall2 (fun e e' => compile e = Some e') es es'.
-induction es; intros0 Heq; simpl in *; invc Heq.
+Lemma I_R_value_fwd : forall LE TE l t,
+    L.value l -> T.value t ->
+    compile_list LE = Some TE ->
+    R LE TE l t -> I LE TE l t.
+induction l using L.expr_ind'; intros0 Lval Tval Henv RR;
+invc Lval; invc RR; invc Tval.
+
+- constructor; eauto.
+  simpl. fold compile_list. unfold seq, fmap.
+
+  assert (forall i,
+    forall l, nth_error args i = Some l ->
+    forall t, nth_error targs i = Some t ->
+    (forall t, L.value l -> T.value t -> compile_list LE = Some TE ->
+        R LE TE l t -> I LE TE l t) ->
+    L.value l -> T.value t ->
+    R LE TE l t ->
+    I LE TE l t) by (intros; eauto).
+  on _, fun H => (assert (Forall2 (I LE TE) args targs) by (list_magic **); clear H).
+  fwd eapply Forall2_I_compile_list as HH; eauto.
+    rewrite HH. clear HH. simpl.
+  reflexivity.
+
+- constructor; eauto.
+  simpl. fold compile_list. unfold seq, fmap.
+
+  assert (forall i,
+    forall l, nth_error free i = Some l ->
+    forall t, nth_error tfree i = Some t ->
+    (forall t, L.value l -> T.value t -> compile_list LE = Some TE ->
+        R LE TE l t -> I LE TE l t) ->
+    L.value l -> T.value t ->
+    R LE TE l t ->
+    I LE TE l t) by (intros; eauto).
+  on _, fun H => (assert (Forall2 (I LE TE) free tfree) by (list_magic **); clear H).
+  fwd eapply Forall2_I_compile_list as HH; eauto.
+    rewrite HH. clear HH. simpl.
+  reflexivity.
+Qed.
+
+Lemma compile_list_Forall2 : forall ls ts,
+    compile_list ls = Some ts ->
+    Forall2 (fun l t => compile l = Some t) ls ts.
+induction ls; intros0 Heq; simpl in *; invc Heq.
 - constructor.
 - compute [seq fmap bind_option] in *.
   destruct (compile _) eqn:?; simpl in *; try discriminate.
@@ -1703,209 +162,451 @@ induction es; intros0 Heq; simpl in *; invc Heq.
   constructor; eauto.
 Qed.
 
+Lemma Forall2_nth_error_exists : forall X Y (P : X -> Y -> Prop) xs ys,
+    Forall2 P xs ys ->
+    forall i x,
+    nth_error xs i = Some x ->
+    exists y, nth_error ys i = Some y /\ P x y.
+intros.
+fwd eapply Forall2_nth_error_Some; eauto. break_exists.
+eexists; split; [ eassumption | ].
+eapply Forall2_nth_error; eauto.
+Qed.
+
+Lemma compile_program_def : forall LE TE l t,
+    compile l = Some t ->
+    compile_list LE = Some TE ->
+    compile_program (l, LE) = Some (t, TE).
+intros0 Heq Heqs.
+unfold compile_program. simpl. rewrite Heq, Heqs. reflexivity.
+Qed.
+
+Lemma I_R_value_rev : forall LE TE l t,
+    L.value l -> T.value t ->
+    compile_list LE = Some TE ->
+    I LE TE l t -> R LE TE l t.
+induction l using L.expr_ind'; intros0 Lval Tval Henv II;
+invc Lval; invc II; invc Tval.
+
+- simpl_compile. break_bind_option. inject_some.
+  constructor.
+  fwd eapply compile_list_Forall2 with (ls := args); eauto.
+
+  assert (forall i,
+    forall l, nth_error args i = Some l ->
+    forall t, nth_error args0 i = Some t ->
+    (forall t, L.value l -> T.value t -> compile_list LE = Some TE ->
+        I LE TE l t -> R LE TE l t) ->
+    L.value l -> T.value t ->
+    compile l = Some t ->
+    R LE TE l t) by (intros; eauto using ICompile).
+  list_magic **.
+
+- simpl_compile. break_bind_option. congruence.
+
+- simpl_compile. break_bind_option. congruence.
+
+- simpl_compile. break_bind_option. inject_some.
+
+  (* TODO: missing premise: l is well formed, no closures with bad fnames *)
+  assert (exists lbody, nth_error LE f0 = Some lbody) by admit. break_exists.
+  fwd eapply compile_list_Forall2 with (ls := LE); eauto.
+  fwd eapply Forall2_nth_error_exists; eauto. break_exists. break_and.
+  fwd eapply compile_list_Forall2 with (ls := free); eauto.
+
+  econstructor; eauto using compile_program_def.
+  assert (forall i,
+    forall l, nth_error free i = Some l ->
+    forall t, nth_error free0 i = Some t ->
+    (forall t, L.value l -> T.value t -> compile_list LE = Some TE ->
+        I LE TE l t -> R LE TE l t) ->
+    L.value l -> T.value t ->
+    compile l = Some t ->
+    R LE TE l t) by (intros; eauto using ICompile).
+  list_magic **.
+
+Admitted.
+
+Lemma I_R_value : forall LE TE l t,
+    L.value l -> T.value t ->
+    compile_list LE = Some TE ->
+    I LE TE l t <-> R LE TE l t.
+intros. split; eauto using I_R_value_fwd, I_R_value_rev.
+Qed.
+
+
 Lemma compile_list_length : forall es es',
     compile_list es = Some es' ->
     length es = length es'.
 intros. eapply Forall2_length. eapply compile_list_Forall2. assumption.
 Qed.
 
-Lemma compile_value : forall le te,
-    L.value le ->
-    compile le = Some te ->
-    T.value te.
-induction le using L.expr_ind'; inversion 1; subst; intros0 Hcomp.
+Lemma compile_R : forall LE TE l t,
+    L.value l ->
+    compile_program (l, LE) = Some (t, TE) ->
+    R LE TE l t.
+induction l using L.expr_ind'; intros0 Lval Hcomp;
+invc Lval;
+unfold compile_program in Hcomp.
 
-- simpl in Hcomp. fold compile_list in Hcomp. unfold seq, fmap in Hcomp.
-  destruct (compile_list args) as [targs|] eqn:?; simpl in Hcomp; try discriminate Hcomp.
-  invc Hcomp.
+- break_bind_option. inject_some. inject_pair.
+  simpl_compile. break_bind_option. inject_some.
+  rename l into targs.
+
   constructor.
+  fwd eapply compile_list_Forall2 with (ls := args); eauto.
 
-  fwd eapply compile_list_Forall2; try eassumption.
   assert (forall i,
-    forall le, nth_error args i = Some le ->
-    forall te, nth_error targs i = Some te ->
-    (forall te, L.value le -> compile le = Some te -> T.value te) ->
-    compile le = Some te ->
-    L.value le ->
-    T.value te) by (intros; eauto).
+    forall l, nth_error args i = Some l ->
+    forall t, nth_error targs i = Some t ->
+    (forall t, L.value l -> compile_program (l, LE) = Some (t, TE) -> R LE TE l t) ->
+    L.value l ->
+    compile l = Some t ->
+    R LE TE l t) by eauto using compile_program_def.
   list_magic **.
 
-- simpl in Hcomp. fold compile_list in Hcomp. unfold seq, fmap in Hcomp.
-  destruct (compile_list free) as [tfree|] eqn:?; simpl in Hcomp; try discriminate Hcomp.
-  invc Hcomp.
-  constructor.
+- break_bind_option. inject_some. inject_pair.
+  simpl_compile. break_bind_option. inject_some.
+  rename l into tfree.
 
-  fwd eapply compile_list_Forall2; try eassumption.
+  (* TODO: missing premise: l is well formed, no closures with bad fnames *)
+  assert (exists lbody, nth_error LE f = Some lbody) by admit.  break_exists.
+  fwd eapply length_nth_error_Some with (ys := TE);
+    try eassumption; eauto using compile_list_length.  break_exists.
+  fwd eapply compile_list_Forall2 with (ls := LE); try eassumption.
+  fwd eapply Forall2_nth_error; try eassumption. cbv beta in *.
+
+  econstructor; eauto using compile_program_def.
+
+  fwd eapply compile_list_Forall2 with (ls := free); try eassumption.
   assert (forall i,
-    forall le, nth_error free i = Some le ->
-    forall te, nth_error tfree i = Some te ->
-    (forall te, L.value le -> compile le = Some te -> T.value te) ->
-    compile le = Some te ->
-    L.value le ->
-    T.value te) by (intros; eauto).
+    forall l, nth_error free i = Some l ->
+    forall t, nth_error tfree i = Some t ->
+    (forall t, L.value l -> compile_program (l, LE) = Some (t, TE) -> R LE TE l t) ->
+    L.value l ->
+    compile l = Some t ->
+    R LE TE l t) by eauto using compile_program_def.
   list_magic **.
 
+Admitted.
+
+
+Lemma R_value : forall LE TE l t,
+    R LE TE l t ->
+    L.value l ->
+    T.value t.
+induction l using L.expr_ind'; intros0 RR Lval; invc Lval; invc RR; constructor.
+
+- assert (forall i,
+    forall l, nth_error args i = Some l ->
+    forall t, nth_error targs i = Some t ->
+    (forall t, R LE TE l t -> L.value l -> T.value t) ->
+    R LE TE l t ->
+    L.value l ->
+    T.value t) by eauto.
+  list_magic **.
+
+- assert (forall i,
+    forall l, nth_error free i = Some l ->
+    forall t, nth_error tfree i = Some t ->
+    (forall t, R LE TE l t -> L.value l -> T.value t) ->
+    R LE TE l t ->
+    L.value l ->
+    T.value t) by eauto.
+  list_magic **.
+
+Qed.
+
+
+Lemma compile_value : forall l t,
+    compile l = Some t ->
+    L.value l ->
+    T.value t.
+intros.
+fwd eapply compile_R with (LE := []) (TE := []); try eassumption.
+  { unfold compile_program. simpl. unfold seq, fmap. rewrite H. reflexivity. }
+eapply R_value; eauto.
 Qed.
 
 Lemma compile_list_value : forall ls ts,
+    compile_list ls = Some ts ->
     Forall L.value ls ->
-    compile_list ls = Some ts ->
     Forall T.value ts.
-induction ls; inversion 1; subst; intros0 Hcomp.
-- simpl in Hcomp. invc Hcomp. constructor.
-- on (Forall _ (_ :: _)), invc.
-  simpl in Hcomp.
-  destruct (compile _) eqn:?; simpl in Hcomp; try discriminate Hcomp.
-  destruct (compile_list _) eqn:?; simpl in Hcomp; try discriminate Hcomp.
-  compute in Hcomp. invc Hcomp.
-  constructor; eauto using compile_value.
+intros.
+fwd eapply compile_list_Forall2; eauto.
+assert (forall i,
+  forall l, nth_error ls i = Some l ->
+  forall t, nth_error ts i = Some t ->
+  compile l = Some t ->
+  L.value l ->
+  T.value t) by eauto using compile_value.
+list_magic **.
 Qed.
 
-Lemma compile_list_nth_error : forall ls ts n le te,
-    compile_list ls = Some ts ->
-    nth_error ls n = Some le ->
-    nth_error ts n = Some te ->
-    compile le = Some te.
-intros. fwd eapply compile_list_Forall2; eauto.
-eapply Forall2_nth_error with (1 := **); eauto.
-Qed.
-
-Ltac inject_some := repeat on (Some _ = Some _), invc.
-Ltac break_bind_option :=
-    repeat match goal with
-    | [ H : bind_option ?x _ = Some _ |- _ ] =>
-            destruct x eqn:?; [ simpl in H | discriminate H ]
-    end.
-
-Theorem subst_compile : forall larg lfree lbody lr  targ tfree tbody tr,
-    compile larg = Some targ ->
-    compile_list lfree = Some tfree ->
-    compile lbody = Some tbody ->
-    L.subst larg lfree lbody = Some lr ->
-    T.subst targ tfree tbody = Some tr ->
-    compile lr = Some tr.
-induction lbody using L.expr_ind'; intros0 Carg Cfree Cbody Lsub Tsub;
-simpl in *; try fold compile_list in *; try fold (L.subst_list larg lfree) in *;
-unfold seq, fmap in *.
-
-- inject_some. assumption.
-- inject_some. simpl in *. eauto using compile_list_nth_error.
-- break_bind_option. inject_some.
-  simpl in *. unfold seq, fmap in *.  break_bind_option. inject_some.
-  fwd eapply (IHlbody1 ?? ?? ?? ?? ?? ** **) as HH; eauto.
-    rewrite HH. clear HH. simpl.
-  fwd eapply (IHlbody2 ?? ?? ?? ?? ?? ** **) as HH; eauto.
-    rewrite HH. clear HH. simpl.
-  reflexivity.
-- break_bind_option. inject_some.
-  simpl in *. fold (T.subst_list targ tfree) in *. fold compile_list.
-  simpl in *. unfold seq, fmap in *.  break_bind_option. inject_some.
-  admit.
-- admit.
-- admit.
-Admitted.
-    
 
 
-Theorem match_states3_sim : forall LE TE le te le',
-    match_states3 LE TE le te ->
-    L.step LE le le' ->
-    exists te', T.step TE te te' /\ match_states3 LE TE le' te'.
-induction le using L.expr_ind'; intros0 Hms Lstep; invc Lstep.
+Definition L_num_upvars :=
+    let fix go e :=
+        let fix go_list es :=
+            match es with
+            | [] => 0
+            | e :: es => max (go e) (go_list es)
+            end in
+        match e with
+        | L.Arg => 0
+        | L.UpVar i => S i
+        | L.Call f a => max (go f) (go a)
+        | L.Constr _ args => go_list args
+        | L.Elim _ cases target => max (go_list cases) (go target)
+        | L.Close _ free => go_list free
+        end in go.
 
-- invc Hms. simpl in H0. fold compile_list in H0. unfold seq, fmap in H0.
-  destruct (compile_list free) as [tfree|] eqn:?; simpl in H0; try discriminate H0.
-  destruct (compile le2) as [te2|] eqn:?; simpl in H0; try discriminate H0.
-  invc H0.
+Definition L_num_upvars_list :=
+    let go := L_num_upvars in
+    let fix go_list es :=
+        match es with
+        | [] => 0
+        | e :: es => max (go e) (go_list es)
+        end in go_list.
 
-  fwd eapply compile_value; eauto.
-  fwd eapply length_nth_error_Some with (ys := TE) as HH;
-    try eassumption; eauto using compile_list_length.
-  destruct HH as [ tbody ? ]. rename e into lbody.
-  fwd eapply compile_list_nth_error with (ls := LE) (ts := TE); eauto.
-  assert (exists te', T.subst te2 tfree tbody = Some te') by admit.  break_exists.
+Ltac refold_L_num_upvars :=
+    fold L_num_upvars_list in *.
 
-  eexists. split; [eapply T.MakeCall | ]; eauto using compile_list_value.
+Ltac L_refold_subst arg vals :=
+    fold (L.subst_list arg vals) in *.
+
+Lemma L_subst_list_Forall2 : forall arg free es es',
+    L.subst_list arg free es = Some es' ->
+    Forall2 (fun e e' => L.subst arg free e = Some e') es es'.
+induction es; intros0 Hsub; destruct es'.
+- constructor.
+- simpl in Hsub. discriminate.
+- simpl in Hsub. break_bind_option. inject_some. discriminate.
+- simpl in Hsub. break_bind_option. inject_some.
+  on (_ :: _ = _ :: _), invc.
   constructor; eauto.
-  eapply subst_compile; [ .. | eassumption | eassumption ]; assumption.
+Qed.
 
-- invc Hms. simpl in H0. unfold seq, fmap in H0.
-  destruct (compile le1) as [te1|] eqn:?; simpl in H0; try discriminate H0.
-  destruct (compile le2) as [te2|] eqn:?; simpl in H0; try discriminate H0.
-  invc H0.
+Lemma L_Forall_num_upvars_list_le : forall es n,
+    Forall (fun e => L_num_upvars e <= n) es ->
+    L_num_upvars_list es <= n.
+induction es; intros0 Hle; simpl in *.
+{ omega. }
+invc Hle.  eapply nat_le_max; eauto.
+Qed.
 
-  assert (match_states3 LE TE le1 te1) by (constructor; assumption).
-  destruct (IHle1 ?? ?? ** **) as (te1' & ? & ?).
+Lemma L_subst_num_upvars : forall arg free body body',
+    L.subst arg free body = Some body' ->
+    L_num_upvars body <= length free.
+induction body using L.expr_ind'; intros0 Hsub;
+simpl in *; refold_L_num_upvars; L_refold_subst arg free.
 
-  eexists. split.  { constructor. eassumption. }
-  repeat on (match_states3 _ _ _ _), invc.
-  constructor; eauto. simpl. unfold seq, fmap.
-  repeat on (compile _ = _), fun H => rewrite H.
+- omega.
+
+- assert (HH : nth_error free n <> None) by congruence.
+  rewrite nth_error_Some in HH.
+  omega.
+
+- break_bind_option. inject_some.
+  specialize (IHbody1 ?? ***).
+  specialize (IHbody2 ?? ***).
+  eauto using nat_le_max.
+
+- break_bind_option. inject_some.
+  fwd eapply L_subst_list_Forall2; try eassumption.
+  rename l into args'.
+  eapply L_Forall_num_upvars_list_le.
+  assert (forall i,
+    forall e, nth_error args i = Some e ->
+    forall e', nth_error args' i = Some e' ->
+    (forall e', L.subst arg free e = Some e' -> L_num_upvars e <= length free) ->
+    L.subst arg free e = Some e' ->
+    L_num_upvars e <= length free) by eauto.
+  list_magic **.
+
+- break_bind_option. inject_some.
+
+  (* target *)
+  specialize (IHbody _ ***). eapply nat_le_max; eauto.
+
+  (* cases *)
+  fwd eapply L_subst_list_Forall2; eauto.
+  rename l into cases'.
+  eapply L_Forall_num_upvars_list_le.
+  assert (forall i,
+    forall e, nth_error cases i = Some e ->
+    forall e', nth_error cases' i = Some e' ->
+    (forall e', L.subst arg free e = Some e' -> L_num_upvars e <= length free) ->
+    L.subst arg free e = Some e' ->
+    L_num_upvars e <= length free) by eauto.
+  list_magic **.
+
+- break_bind_option. inject_some.
+  fwd eapply L_subst_list_Forall2; try eassumption.
+  rename free0 into es.
+  rename l into es'.
+  eapply L_Forall_num_upvars_list_le.
+  assert (forall i,
+    forall e, nth_error es i = Some e ->
+    forall e', nth_error es' i = Some e' ->
+    (forall e', L.subst arg free e = Some e' -> L_num_upvars e <= length free) ->
+    L.subst arg free e = Some e' ->
+    L_num_upvars e <= length free) by eauto.
+  list_magic **.
+
+Qed.
+
+
+Lemma compile_num_upvars : forall l t,
+    compile l = Some t ->
+    L_num_upvars l = T_num_upvars t.
+induction l using L.expr_ind'; intros0 Hcomp;
+simpl_compile; refold_L_num_upvars.
+
+- inject_some. simpl. reflexivity.
+
+- inject_some. simpl. reflexivity.
+
+- break_bind_option. inject_some.
+  specialize (IHl1 _ ***). find_rewrite.
+  specialize (IHl2 _ ***). find_rewrite.
   simpl. reflexivity.
 
-- admit.
-
-- admit.
-
-- admit.
-
-- admit.
-
-- admit.
-
-Admitted.
-
-
-Theorem match_states3_rel : forall LE TE le te,
-    match_states3 LE TE le te ->
-    L.value le -> T.value te ->
-    rel LE TE le te.
-induction le using L.expr_ind';
-intros0 Hms Lval Tval; invc Lval; invc Tval.
-
-Focus 2. {
-      exfalso. invc Hms. simpl in *. unfold seq, fmap in *.
-      break_bind_option. congruence.
-} Unfocus.
-Focus 2. {
-      exfalso. invc Hms. simpl in *. unfold seq, fmap in *.
-      break_bind_option. congruence.
-} Unfocus.
-
-- invc Hms. simpl in *. fold compile_list in *.
-  unfold seq, fmap in *. break_bind_option. inject_some.
-  constructor.
-  fwd eapply compile_list_Forall2; eauto.
+- break_bind_option. inject_some. simpl. refold_T_num_upvars.
   admit.
 
-- invc Hms. simpl in *. fold compile_list in *.
-  unfold seq, fmap in *. break_bind_option. inject_some.
+- admit.
 
-  assert (exists lbody, nth_error LE f0 = Some lbody) by admit.  break_exists.
-  assert (exists tbody, nth_error TE f0 = Some tbody) by admit.  break_exists.
-    (* missing premises: le/te are well formed, no Calls to bad fnames *)
-  fwd eapply compile_list_nth_error with (ls := LE) (ts := TE); eauto.
+- admit.
+Admitted.
 
-  eapply RClose with (rename := id); eauto.
 
-  + unfold compile_program, seq, fmap. simpl.
-    on (compile _ = Some _), fun H => rewrite H.  simpl.
-    on (compile_list _ = Some _), fun H => rewrite H.  simpl.
-    reflexivity.
+Theorem I_sim : forall LE TE l l' t,
+    I LE TE l t ->
+    L.step LE l l' ->
+    exists t',
+        T.step TE t t' /\
+        I LE TE l' t'.
+induction l using L.expr_ind'; intros0 II Lstep;
+invc Lstep; invc II; simpl_compile; break_bind_option; inject_some.
 
-  + admit. (* program is equivalent to itself under identity renaming *)
+- (* MakeCall *)
+  fwd eapply length_nth_error_Some with (ys := TE); try eassumption.
+    { eauto using compile_list_length. }
+  break_exists.
 
-  + fwd eapply compile_list_Forall2; eauto.
-    assert (forall i,
-        forall le, nth_error free i = Some le ->
-        forall te, nth_error free0 i = Some te ->
-        (forall te, match_states3 LE TE le te -> L.value le -> T.value te -> rel LE TE le te) ->
-        L.value le ->
-        T.value te ->
-        compile le = Some te ->
-        rel LE TE le te). {
-      intros. on _, fun H => eapply H; eauto.  constructor; eauto.
-    }
-    list_magic **.
+  fwd eapply compile_list_Forall2 with (ls := LE) (ts := TE); eauto.
+  fwd eapply Forall2_nth_error; eauto. cbv beta in *.
+
+  rename l into tfree.
+  rename e1 into t2.
+  rename x into te.
+  fwd eapply T_num_upvars_subst with (arg := t2) (free := tfree) (body := te).
+    { erewrite <- compile_num_upvars by eauto.
+      erewrite <- compile_list_length by eauto.
+      eapply L_subst_num_upvars; eauto. }
+  break_exists.
+
+  eexists. split. eapply T.MakeCall; eauto.
+  + eauto using compile_value.
+  + eauto using compile_list_value.
+  + admit. (* subst preserves I *)
+
+- admit.
+- admit.
+- admit.
+- admit.
+- admit.
+- admit.
 
 Admitted.
+
+Lemma I_sim_star : forall LE l l',
+    L.star LE l l' ->
+    forall TE t,
+    I LE TE l t ->
+    exists t',
+        T.star TE t t' /\
+        I LE TE l' t'.
+induction 1; intros0 II.
+- (* nil *) exists t. split; [ constructor | assumption ].
+- (* cons *)
+  fwd eapply I_sim; eauto. break_exists. break_and.
+  specialize (IHstar _ _ **). break_exists. break_and.
+  eexists. split; [ | eassumption ]. econstructor; eassumption.
+Qed.
+
+Lemma I_value : forall LE TE l t,
+    I LE TE l t ->
+    L.value l ->
+    T.value t.
+induction l using L.expr_ind'; intros0 II Lval;
+invc Lval; invc II; simpl_compile; break_bind_option; inject_some.
+
+- constructor.
+  fwd eapply compile_list_Forall2; eauto.
+
+  rename l into targs.
+  assert (forall i,
+    forall l, nth_error args i = Some l ->
+    forall t, nth_error targs i = Some t ->
+    (forall t, I LE TE l t -> L.value l -> T.value t) ->
+    compile l = Some t ->
+    L.value l ->
+    T.value t) by (intros; eauto using ICompile).
+  list_magic **.
+
+- constructor.
+  fwd eapply compile_list_Forall2; eauto.
+
+  rename l into tfree.
+  assert (forall i,
+    forall l, nth_error free i = Some l ->
+    forall t, nth_error tfree i = Some t ->
+    (forall t, I LE TE l t -> L.value l -> T.value t) ->
+    compile l = Some t ->
+    L.value l ->
+    T.value t) by (intros; eauto using ICompile).
+  list_magic **.
+Qed.
+
+Theorem R_compile : forall LE TE l l' t,
+    compile_program (l, LE) = Some (t, TE) ->
+    L.value l' ->
+    L.star LE l l' ->
+    exists t',
+        T.star TE t t' /\
+        T.value t' /\
+        R LE TE l' t'.
+intros0 Hcomp Lval Lstar.
+unfold compile_program in *. break_bind_option. inject_some. inject_pair. simpl in *.
+fwd eapply ICompile; eauto.
+fwd eapply I_sim_star; eauto. break_exists. break_and.
+fwd eapply I_value; eauto.
+rewrite I_R_value in * by eauto.
+eexists; eauto.
+Qed.
+
+Theorem R_call : forall LE TE lf la lr tf ta,
+    compile_list LE = Some TE ->
+    L.value lf -> L.value la -> L.value lr ->
+    T.value tf -> T.value ta ->
+    R LE TE lf tf ->
+    R LE TE la ta ->
+    L.star LE (L.Call lf la) lr ->
+    exists tr,
+        T.star TE (T.Call tf ta) tr /\
+        T.value tr /\
+        R LE TE lr tr.
+intros0 Henv Lvalf Lvala Lvalr Tvalf Tvala RRf RRa Lstar.
+
+assert (compile (L.Call lf la) = Some (T.Call tf ta)). {
+  rewrite <- I_R_value in * by eauto. invc RRf. invc RRa.
+  simpl_compile. repeat find_rewrite.
+  unfold seq, fmap. simpl. reflexivity.
+}
+
+fwd eapply I_sim_star; eauto using ICompile. break_exists. break_and.
+
+eexists; split; [ | split ]; eauto using I_value, I_R_value_rev.
+Qed.
